@prefix : <http://www.semanticweb.org/sylvain/ontologies/2024/9/untitled-ontology-15#> .
@prefix owl: <http://www.w3.org/2002/07/owl#> .
@prefix rdf: <http://www.w3.org/1999/02/22-rdf-syntax-ns#> .
@prefix xml: <http://www.w3.org/XML/1998/namespace> .
@prefix xsd: <http://www.w3.org/2001/XMLSchema#> .
@prefix rdfs: <http://www.w3.org/2000/01/rdf-schema#> .
@base <http://www.semanticweb.org/sylvain/ontologies/2024/9/untitled-ontology-15> .

<http://www.semanticweb.org/sylvain/ontologies/2024/9/untitled-ontology-15> rdf:type owl:Ontology .

#################################################################
#    Annotation properties
#################################################################

###  http://www.w3.org/2004/02/skos/core#changeNote
<http://www.w3.org/2004/02/skos/core#changeNote> rdf:type owl:AnnotationProperty .


###  http://www.w3.org/2004/02/skos/core#scopeNote
<http://www.w3.org/2004/02/skos/core#scopeNote> rdf:type owl:AnnotationProperty .


###  https://www.ica.org/standards/RiC/ontology#RiCCMCorrespondingComponent
<https://www.ica.org/standards/RiC/ontology#RiCCMCorrespondingComponent> rdf:type owl:AnnotationProperty .


###  https://www.ica.org/standards/RiC/ontology#closeTo
<https://www.ica.org/standards/RiC/ontology#closeTo> rdf:type owl:AnnotationProperty .


#################################################################
#    Object Properties
#################################################################

###  https://www.ica.org/standards/RiC/ontology#documentedBy
<https://www.ica.org/standards/RiC/ontology#documentedBy> rdf:type owl:ObjectProperty ;
                                                          rdfs:subPropertyOf <https://www.ica.org/standards/RiC/ontology#isOrganicOrFunctionalProvenanceOf> ,
                                                                             <https://www.ica.org/standards/RiC/ontology#resultsOrResultedIn> ;
                                                          owl:inverseOf <https://www.ica.org/standards/RiC/ontology#documents> ;
                                                          rdfs:domain <https://www.ica.org/standards/RiC/ontology#Activity> ;
                                                          rdfs:range [ rdf:type owl:Class ;
                                                                       owl:unionOf ( <https://www.ica.org/standards/RiC/ontology#Instantiation>
                                                                                     <https://www.ica.org/standards/RiC/ontology#RecordResource>
                                                                                   )
                                                                     ] ;
                                                          rdfs:comment "Inverse of 'documents' object property."@en ;
                                                          rdfs:isDefinedBy <https://www.ica.org/standards/RiC/ontology> ;
                                                          rdfs:label "documented by"@en ,
                                                                     "est documenté par"@fr ,
                                                                     "se documenta en"@es ;
                                                          <http://www.w3.org/2004/02/skos/core#changeNote> [ ] ,
[ ] ,
[ ] ,
[ ] ,
[ ] ;
<https://www.ica.org/standards/RiC/ontology#RiCCMCorrespondingComponent> """RiC-R033i ('documented by'
            relation)"""@en .


###  https://www.ica.org/standards/RiC/ontology#documents
<https://www.ica.org/standards/RiC/ontology#documents> rdf:type owl:ObjectProperty .


###  https://www.ica.org/standards/RiC/ontology#hadComponent
<https://www.ica.org/standards/RiC/ontology#hadComponent> rdf:type owl:ObjectProperty ;
                                                          rdfs:subPropertyOf <https://www.ica.org/standards/RiC/ontology#hadPart> ,
                                                                             <https://www.ica.org/standards/RiC/ontology#hasOrHadComponent> ;
                                                          owl:inverseOf <https://www.ica.org/standards/RiC/ontology#wasComponentOf> ;
                                                          rdfs:domain <https://www.ica.org/standards/RiC/ontology#Instantiation> ;
                                                          rdfs:range <https://www.ica.org/standards/RiC/ontology#Instantiation> ;
                                                          rdfs:comment """Connects an Instantiation to another Instantiation that was its
            component in the past."""@en ;
                                                          rdfs:isDefinedBy <https://www.ica.org/standards/RiC/ontology> ;
                                                          rdfs:label "a eu pour composant"@fr ,
                                                                     "had component"@en ,
                                                                     "tenía como componente"@es ;
                                                          <http://www.w3.org/2004/02/skos/core#changeNote> [ ] ,
[ ] ,
[ ] .


###  https://www.ica.org/standards/RiC/ontology#hadPart
<https://www.ica.org/standards/RiC/ontology#hadPart> rdf:type owl:ObjectProperty .


###  https://www.ica.org/standards/RiC/ontology#hasComponentTransitive
<https://www.ica.org/standards/RiC/ontology#hasComponentTransitive> rdf:type owl:ObjectProperty ;
                                                                    owl:inverseOf <https://www.ica.org/standards/RiC/ontology#isComponentOfTransitive> .


###  https://www.ica.org/standards/RiC/ontology#hasOrHadComponent
<https://www.ica.org/standards/RiC/ontology#hasOrHadComponent> rdf:type owl:ObjectProperty .


###  https://www.ica.org/standards/RiC/ontology#hasOrHadLanguage
<https://www.ica.org/standards/RiC/ontology#hasOrHadLanguage> rdf:type owl:ObjectProperty ;
                                                              owl:inverseOf <https://www.ica.org/standards/RiC/ontology#isOrWasLanguageOf> .


###  https://www.ica.org/standards/RiC/ontology#isAssociatedWithEvent
<https://www.ica.org/standards/RiC/ontology#isAssociatedWithEvent> rdf:type owl:ObjectProperty .


###  https://www.ica.org/standards/RiC/ontology#isComponentOfTransitive
<https://www.ica.org/standards/RiC/ontology#isComponentOfTransitive> rdf:type owl:ObjectProperty ;
                                                                     rdfs:subPropertyOf <https://www.ica.org/standards/RiC/ontology#isOrWasComponentOf> ,
                                                                                        <https://www.ica.org/standards/RiC/ontology#isPartOfTransitive> ;
                                                                     rdf:type owl:TransitiveProperty ;
                                                                     rdfs:domain <https://www.ica.org/standards/RiC/ontology#Instantiation> ;
                                                                     rdfs:range <https://www.ica.org/standards/RiC/ontology#Instantiation> ;
                                                                     rdfs:comment """Connects an Instantiation to another Instantiation of which it
            is, directly or indirectly, a component. This is a transitive relation."""@en ;
                                                                     rdfs:isDefinedBy <https://www.ica.org/standards/RiC/ontology> ;
                                                                     rdfs:label "es componente de transitivo"@es ,
                                                                                "est un composant de transitif"@fr ,
                                                                                "is component of transitive"@en ;
                                                                     <http://www.w3.org/2004/02/skos/core#changeNote> [ ] ,
[ ] ,
[ ] .


###  https://www.ica.org/standards/RiC/ontology#isDateAssociatedWith
<https://www.ica.org/standards/RiC/ontology#isDateAssociatedWith> rdf:type owl:ObjectProperty .


###  https://www.ica.org/standards/RiC/ontology#isDateOfOccurrenceOf
<https://www.ica.org/standards/RiC/ontology#isDateOfOccurrenceOf> rdf:type owl:ObjectProperty ;
                                                                  rdfs:subPropertyOf <https://www.ica.org/standards/RiC/ontology#isAssociatedWithEvent> ,
                                                                                     <https://www.ica.org/standards/RiC/ontology#isDateAssociatedWith> ;
                                                                  owl:inverseOf <https://www.ica.org/standards/RiC/ontology#occurredAtDate> ;
                                                                  rdfs:domain <https://www.ica.org/standards/RiC/ontology#Date> ;
                                                                  rdfs:range <https://www.ica.org/standards/RiC/ontology#Event> ;
                                                                  rdfs:comment """Connects a Date to an Event that occurred at this Date. An event
            or activity can be recurrent, which implies that one single event can be related to
            several dates."""@en ;
                                                                  rdfs:isDefinedBy <https://www.ica.org/standards/RiC/ontology> ;
                                                                  rdfs:label "es fecha de ocurrencia de"@es ,
                                                                             "est la date d'occurrence de"@fr ,
                                                                             "is date of occurrence of"@en ;
                                                                  <http://www.w3.org/2004/02/skos/core#changeNote> [ ] ,
[ ] ,
[ ] ,
[ ] ;
<https://www.ica.org/standards/RiC/ontology#RiCCMCorrespondingComponent> """RiC-R084 ('is date of occurrence of'
            relation)"""@en .


###  https://www.ica.org/standards/RiC/ontology#isOrWasComponentOf
<https://www.ica.org/standards/RiC/ontology#isOrWasComponentOf> rdf:type owl:ObjectProperty .


###  https://www.ica.org/standards/RiC/ontology#isOrWasLanguageOf
<https://www.ica.org/standards/RiC/ontology#isOrWasLanguageOf> rdf:type owl:ObjectProperty ;
                                                               rdfs:subPropertyOf <https://www.ica.org/standards/RiC/ontology#isRelatedTo> ;
                                                               rdfs:domain <https://www.ica.org/standards/RiC/ontology#Language> ;
                                                               rdfs:range [ rdf:type owl:Class ;
                                                                            owl:unionOf ( <https://www.ica.org/standards/RiC/ontology#Agent>
                                                                                          <https://www.ica.org/standards/RiC/ontology#Record>
                                                                                          <https://www.ica.org/standards/RiC/ontology#RecordPart>
                                                                                        )
                                                                          ] ;
                                                               rdfs:comment """Connects a Language to an Agent, Record or Record Part that uses
            or used it."""@en ;
                                                               rdfs:isDefinedBy <https://www.ica.org/standards/RiC/ontology> ;
                                                               rdfs:label "es o era lengua de"@es ,
                                                                          "est ou a été la langue de"@fr ,
                                                                          "is or was language of"@en ;
                                                               <http://www.w3.org/2004/02/skos/core#changeNote> [ ] ,
[ ] ,
[ ] .


###  https://www.ica.org/standards/RiC/ontology#isOrganicOrFunctionalProvenanceOf
<https://www.ica.org/standards/RiC/ontology#isOrganicOrFunctionalProvenanceOf> rdf:type owl:ObjectProperty .


###  https://www.ica.org/standards/RiC/ontology#isPartOfTransitive
<https://www.ica.org/standards/RiC/ontology#isPartOfTransitive> rdf:type owl:ObjectProperty .


###  https://www.ica.org/standards/RiC/ontology#isRelatedTo
<https://www.ica.org/standards/RiC/ontology#isRelatedTo> rdf:type owl:ObjectProperty .


###  https://www.ica.org/standards/RiC/ontology#occurredAtDate
<https://www.ica.org/standards/RiC/ontology#occurredAtDate> rdf:type owl:ObjectProperty .


###  https://www.ica.org/standards/RiC/ontology#performanceRelation_role
<https://www.ica.org/standards/RiC/ontology#performanceRelation_role> rdf:type owl:ObjectProperty .


###  https://www.ica.org/standards/RiC/ontology#recordResourceToInstantiationRelation_role
<https://www.ica.org/standards/RiC/ontology#recordResourceToInstantiationRelation_role> rdf:type owl:ObjectProperty .


###  https://www.ica.org/standards/RiC/ontology#relationHasSource
<https://www.ica.org/standards/RiC/ontology#relationHasSource> rdf:type owl:ObjectProperty .


###  https://www.ica.org/standards/RiC/ontology#relationHasTarget
<https://www.ica.org/standards/RiC/ontology#relationHasTarget> rdf:type owl:ObjectProperty .


###  https://www.ica.org/standards/RiC/ontology#resultsOrResultedIn
<https://www.ica.org/standards/RiC/ontology#resultsOrResultedIn> rdf:type owl:ObjectProperty .


###  https://www.ica.org/standards/RiC/ontology#temporalRelation_role
<https://www.ica.org/standards/RiC/ontology#temporalRelation_role> rdf:type owl:ObjectProperty .


###  https://www.ica.org/standards/RiC/ontology#wasComponentOf
<https://www.ica.org/standards/RiC/ontology#wasComponentOf> rdf:type owl:ObjectProperty ;
                                                            rdfs:subPropertyOf <https://www.ica.org/standards/RiC/ontology#isOrWasComponentOf> ,
                                                                               <https://www.ica.org/standards/RiC/ontology#wasPartOf> ;
                                                            rdfs:domain <https://www.ica.org/standards/RiC/ontology#Instantiation> ;
                                                            rdfs:range <https://www.ica.org/standards/RiC/ontology#Instantiation> ;
                                                            rdfs:comment """Connects an Instantiation to another Instantiation of which it
            was a component in the past."""@en ;
                                                            rdfs:isDefinedBy <https://www.ica.org/standards/RiC/ontology> ;
                                                            rdfs:label "a été le composant de"@fr ,
                                                                       "era componente de"@es ,
                                                                       "was component of"@en ;
                                                            <http://www.w3.org/2004/02/skos/core#changeNote> [ ] ,
[ ] ,
[ ] .


###  https://www.ica.org/standards/RiC/ontology#wasPartOf
<https://www.ica.org/standards/RiC/ontology#wasPartOf> rdf:type owl:ObjectProperty .


#################################################################
#    Classes
#################################################################

###  https://www.ica.org/standards/RiC/ontology#Activity
<https://www.ica.org/standards/RiC/ontology#Activity> rdf:type owl:Class ;
                                                      rdfs:subClassOf <https://www.ica.org/standards/RiC/ontology#Event> ;
                                                      rdfs:comment "The doing of something for some human purpose."@en ;
                                                      rdfs:isDefinedBy <https://www.ica.org/standards/RiC/ontology> ;
                                                      rdfs:label "Actividad"@es ,
                                                                 "Activity"@en ,
                                                                 "Activité"@fr ;
                                                      <http://www.w3.org/2004/02/skos/core#changeNote> [ ] ,
[ ] ,
[ ] ,
[ ] ;
<http://www.w3.org/2004/02/skos/core#scopeNote> """Activity is a kind of Event. Activity is specifically used to
            designate purposeful human activity. Activity may be understood from two perspectives.
            First it can be understood as leading to an end. The end is the purpose of the Activity,
            or why the Activity is performed. Second, it can be understood in terms of the processes
            that lead to achieving the end, how the end is realized through coordinated actions.
            Purpose and process are complementary understandings of Activity. Together the two
            perspectives address why the Activity is performed, the expected ends or outcomes; and
            how the Activity fulfills the purpose. While activity has an intended end, it also has
            unintended consequences and results, or side-effects. By and large, these may not be the
            focus of the description, but they are, unquestionably, context. |In a corporate or
            government context an Activity may also be called a 'function'. An Activity exists in a
            specific social and cultural context, and within that context is subject to change over
            time. An Activity may be composed of other Activities."""@en ;
<https://www.ica.org/standards/RiC/ontology#RiCCMCorrespondingComponent> """Corresponds to RiC-E15 (Activity
            entity)"""@en .


###  https://www.ica.org/standards/RiC/ontology#ActivityType
<https://www.ica.org/standards/RiC/ontology#ActivityType> rdf:type owl:Class ;
                                                          rdfs:subClassOf <https://www.ica.org/standards/RiC/ontology#Type> ;
                                                          rdfs:comment "Categorization of an Activity."@en ;
                                                          rdfs:isDefinedBy <https://www.ica.org/standards/RiC/ontology> ;
                                                          rdfs:label "Activity Type"@en ,
                                                                     "Tipo de actividad"@es ,
                                                                     "Type d’activité"@fr ;
                                                          <http://www.w3.org/2004/02/skos/core#changeNote> [ ] ,
[ ] ,
[ ] ,
[ ] ;
<http://www.w3.org/2004/02/skos/core#scopeNote> """Can be extended with any number of subclasses, e.g.
            “function/action” and “activity domain”. This allows for a faceted approach that enables
            an Activity to be categorized using a combination of components, general or more
            specific. For example, “monitoring” can be used in combination with “election polls” or
            “water resources”."""@en ;
<https://www.ica.org/standards/RiC/ontology#RiCCMCorrespondingComponent> """Corresponds to RiC-A02 (Activity Type
            attribute)"""@en .


###  https://www.ica.org/standards/RiC/ontology#Agent
<https://www.ica.org/standards/RiC/ontology#Agent> rdf:type owl:Class ;
                                                   rdfs:subClassOf <https://www.ica.org/standards/RiC/ontology#Thing> ;
                                                   rdfs:comment """A Person, or Group, or an entity created by a Person or Group
            (Mechanism), or a Position, that acts in the world."""@en ;
                                                   rdfs:isDefinedBy <https://www.ica.org/standards/RiC/ontology> ;
                                                   rdfs:label "Agent"@en ,
                                                              "Agent"@fr ,
                                                              "Agente"@es ;
                                                   <http://www.w3.org/2004/02/skos/core#changeNote> [ ] ,
[ ] ,
[ ] ,
[ ] ;
<http://www.w3.org/2004/02/skos/core#scopeNote> """An Agent may have one or more identities; an identity is a
            constellation of properties or relations that together “identify” the Agent. A Person or
            Group commonly has one identity, though each also may have one or more alternative
            identities. Such alternative identities may be shared by more than one Person or Group.
            Alternative identities include but are not limited to pseudonyms, heteronyms, DBA (Doing
            Business As), and trade identities. An alternative identity should not be confused with
            a Position in a Group, for example, presidents, prime ministers, governors, popes,
            royalty, or bishops. Nor should an alternative identity be confused with a variant name
            or identifier of the same identity. Agent also includes entities created by a Person or
            Group that act on behalf of the creating Agent in an autonomous or semi-autonomous
            manner. Examples of a Mechanism include software agents, robots, and space and
            underwater probes that generate data (records) in the course of Activity assigned to and
            in conformance with the instructions given to them by the creating Person or
            Group."""@en ;
<https://www.ica.org/standards/RiC/ontology#RiCCMCorrespondingComponent> """Corresponds to RiC-E07 (Agent
            entity)"""@en .


###  https://www.ica.org/standards/RiC/ontology#Appellation
<https://www.ica.org/standards/RiC/ontology#Appellation> rdf:type owl:Class ;
                                                         rdfs:subClassOf <https://www.ica.org/standards/RiC/ontology#Concept> ;
                                                         rdfs:comment """A concept of any kind that is used for designating an Entity and
            referring to it."""@en ;
                                                         rdfs:isDefinedBy <https://www.ica.org/standards/RiC/ontology> ;
                                                         rdfs:label "Appellation"@en ,
                                                                    "Appellation"@fr ,
                                                                    "Denominación"@es ;
                                                         <http://www.w3.org/2004/02/skos/core#changeNote> [ ] ,
[ ] .


###  https://www.ica.org/standards/RiC/ontology#Concept
<https://www.ica.org/standards/RiC/ontology#Concept> rdf:type owl:Class .


###  https://www.ica.org/standards/RiC/ontology#ContentType
<https://www.ica.org/standards/RiC/ontology#ContentType> rdf:type owl:Class ;
                                                         rdfs:subClassOf <https://www.ica.org/standards/RiC/ontology#Type> ;
                                                         rdfs:comment """The fundamental form of communication in which a Record or
            Record Part is expressed."""@en ;
                                                         rdfs:isDefinedBy <https://www.ica.org/standards/RiC/ontology> ;
                                                         rdfs:label "Content Type"@en ,
                                                                    "Tipo de contenido"@es ,
                                                                    "Type de contenu"@fr ;
                                                         <http://www.w3.org/2004/02/skos/core#changeNote> [ ] ,
[ ] ,
[ ] ,
[ ] ,
[ ] ;
<http://www.w3.org/2004/02/skos/core#scopeNote> """Content Type should not be confused with Representation Type
            or Carrier Type that would concern a related Instantiation since the form of
            communication can be independent of the representation or carrier, for example a map
            (content type \"cartographic image\") may be represented as a sketch (representation type
            \"visual\") recorded as a physical document (carrier type \"paper\"). It also should not be
            confused with the Documentary Form Type of a Record, or Record Part, which describes a
            specific document form (for example a deed of sale)."""@en ;
<https://www.ica.org/standards/RiC/ontology#RiCCMCorrespondingComponent> """Corresponds to RiC-A10 (Content Type
            attribute)"""@en .


###  https://www.ica.org/standards/RiC/ontology#Coordinates
<https://www.ica.org/standards/RiC/ontology#Coordinates> rdf:type owl:Class ;
                                                         rdfs:subClassOf <https://www.ica.org/standards/RiC/ontology#Thing> ;
                                                         rdfs:comment """Longitudinal and latitudinal information about a
            Place."""@en ;
                                                         rdfs:isDefinedBy <https://www.ica.org/standards/RiC/ontology> ;
                                                         rdfs:label "Coordenadas de lugar"@es ,
                                                                    "Coordinates"@en ,
                                                                    "Coordonnées géographiques"@fr ;
                                                         <http://www.w3.org/2004/02/skos/core#changeNote> [ ] ,
[ ] ,
[ ] ,
[ ] ,
[ ] ;
<https://www.ica.org/standards/RiC/ontology#RiCCMCorrespondingComponent> """Class implementation of RiC-A11 (Coordinates
            attribute)"""@en .


###  https://www.ica.org/standards/RiC/ontology#Date
<https://www.ica.org/standards/RiC/ontology#Date> rdf:type owl:Class ;
                                                  rdfs:subClassOf <https://www.ica.org/standards/RiC/ontology#Thing> ;
                                                  rdfs:comment """Chronological information associated with an entity that
            contributes to its identification and contextualization."""@en ;
                                                  rdfs:isDefinedBy <https://www.ica.org/standards/RiC/ontology> ;
                                                  rdfs:label "Date"@en ,
                                                             "Date"@fr ,
                                                             "Fecha"@es ;
                                                  <http://www.w3.org/2004/02/skos/core#changeNote> [ ] ,
[ ] ,
[ ] ,
[ ] ;
<http://www.w3.org/2004/02/skos/core#scopeNote> """A Date may be represented in natural language, based on a
            digital standard, or both. Digital standard dates will typically be based on ISO 8601,
            or Extended Date-Time Format (EDTF)"""@en ;
<https://www.ica.org/standards/RiC/ontology#RiCCMCorrespondingComponent> """Corresponds to RiC-E18 (Date
            entity)"""@en .


###  https://www.ica.org/standards/RiC/ontology#DateType
<https://www.ica.org/standards/RiC/ontology#DateType> rdf:type owl:Class ;
                                                      rdfs:subClassOf <https://www.ica.org/standards/RiC/ontology#Type> ;
                                                      rdfs:comment "Categorization of a Date."@en ;
                                                      rdfs:isDefinedBy <https://www.ica.org/standards/RiC/ontology> ;
                                                      rdfs:label "Date Type"@en ,
                                                                 "Tipo de fecha"@es ,
                                                                 "Type de date"@fr ;
                                                      <http://www.w3.org/2004/02/skos/core#changeNote> [ ] ,
[ ] ,
[ ] ;
<http://www.w3.org/2004/02/skos/core#scopeNote> """May be used to categorize a Date as a single date, a date
            range or a date set or sub-categories of these broad types. This attribute should not be
            confused with the date relations defined to connect a Date entity and any other entity
            (such as RiC-R069 ‘is beginning date of’)."""@en ;
<https://www.ica.org/standards/RiC/ontology#RiCCMCorrespondingComponent> """Corresponds to RiC-A42 (Date Type attribute) (new
            in RiC-CM 1.0)."""@en .


###  https://www.ica.org/standards/RiC/ontology#DocumentaryFormType
<https://www.ica.org/standards/RiC/ontology#DocumentaryFormType> rdf:type owl:Class ;
                                                                 rdfs:subClassOf <https://www.ica.org/standards/RiC/ontology#Type> ;
                                                                 rdfs:comment """Categorization of a Record or Record Part with respect to its
            extrinsic and intrinsic elements that together communicate its content, administrative
            and documentary context, and authority."""@en ;
                                                                 rdfs:isDefinedBy <https://www.ica.org/standards/RiC/ontology> ;
                                                                 rdfs:label "Documentary Form Type"@en ,
                                                                            "Tipo documental"@es ,
                                                                            "Type de document"@fr ;
                                                                 <http://www.w3.org/2004/02/skos/core#changeNote> [ ] ,
[ ] ,
[ ] ,
[ ] ,
[ ] ;
<http://www.w3.org/2004/02/skos/core#scopeNote> """Documentary Form Type plays an important role in determining
            the type of information a Record may comprise, its status of perfection, and its
            authenticity and reliability. Documentary form types exist in a specific social and
            cultural context, and within that context, are subject to change over
            time."""@en ;
<https://www.ica.org/standards/RiC/ontology#RiCCMCorrespondingComponent> """Corresponds to RiC-A17 (Documentary Form Type
            attribute)"""@en .


###  https://www.ica.org/standards/RiC/ontology#Event
<https://www.ica.org/standards/RiC/ontology#Event> rdf:type owl:Class .


###  https://www.ica.org/standards/RiC/ontology#EventRelation
<https://www.ica.org/standards/RiC/ontology#EventRelation> rdf:type owl:Class .


###  https://www.ica.org/standards/RiC/ontology#EventType
<https://www.ica.org/standards/RiC/ontology#EventType> rdf:type owl:Class ;
                                                       rdfs:subClassOf <https://www.ica.org/standards/RiC/ontology#Type> ;
                                                       rdfs:comment "Categorization of an Event."@en ;
                                                       rdfs:isDefinedBy <https://www.ica.org/standards/RiC/ontology> ;
                                                       rdfs:label "Event Type"@en ,
                                                                  "Tipo de evento"@es ,
                                                                  "Type d’événement"@fr ;
                                                       <http://www.w3.org/2004/02/skos/core#changeNote> [ ] ,
[ ] ,
[ ] ,
[ ] ,
[ ] ;
<http://www.w3.org/2004/02/skos/core#scopeNote> """Events of all kinds can be categorized. Curation event types
            include creation; acquisition; transfer; arrangement; description; digitization, etc.
            Biographical event types include birth, marriage, death, etc."""@en ;
<https://www.ica.org/standards/RiC/ontology#RiCCMCorrespondingComponent> """Corresponds to RiC-A18 (Event Type
            attribute)"""@en .


###  https://www.ica.org/standards/RiC/ontology#Group
<https://www.ica.org/standards/RiC/ontology#Group> rdf:type owl:Class ;
                                                   owl:disjointWith <https://www.ica.org/standards/RiC/ontology#Person> .


###  https://www.ica.org/standards/RiC/ontology#Identifier
<https://www.ica.org/standards/RiC/ontology#Identifier> rdf:type owl:Class ;
                                                        rdfs:subClassOf <https://www.ica.org/standards/RiC/ontology#Appellation> ;
                                                        rdfs:comment """A word, number, letter, symbol, or any combination of these used
            to uniquely identify or reference an individual instance of an entity within a specific
            information domain."""@en ;
                                                        rdfs:isDefinedBy <https://www.ica.org/standards/RiC/ontology> ;
                                                        rdfs:label "Identifiant"@fr ,
                                                                   "Identificador"@es ,
                                                                   "Identifier"@en ;
                                                        <http://www.w3.org/2004/02/skos/core#changeNote> [ ] ,
[ ] ,
[ ] ,
[ ] ;
<http://www.w3.org/2004/02/skos/core#scopeNote> """Can include Global Persistent Identifiers (globally unique and
            persistently resolvable identifier for the entity) and/or Local Identifiers. Both the
            domain within which the identifier is unique, and the rules used in forming the
            identifier value should be provided with the identifier value."""@en ;
<https://www.ica.org/standards/RiC/ontology#RiCCMCorrespondingComponent> """Class implementation of RiC-A22 (Identifier
            attribute) (see also the identifier datatype property)"""@en .


###  https://www.ica.org/standards/RiC/ontology#IdentifierType
<https://www.ica.org/standards/RiC/ontology#IdentifierType> rdf:type owl:Class ;
                                                            rdfs:subClassOf <https://www.ica.org/standards/RiC/ontology#Type> ;
                                                            rdfs:comment "Categorization of an Identifier."@en ;
                                                            rdfs:isDefinedBy <https://www.ica.org/standards/RiC/ontology> ;
                                                            rdfs:label "Identifier Type"@en ,
                                                                       "Tipo de identificador"@es ,
                                                                       "Type d’identifiant"@fr ;
                                                            <http://www.w3.org/2004/02/skos/core#changeNote> [ ] ,
[ ] ,
[ ] ,
[ ] ;
<http://www.w3.org/2004/02/skos/core#scopeNote> """For example, 'old identifier' ; 'ISNI' (for a person or
            corporate body), etc."""@en .


###  https://www.ica.org/standards/RiC/ontology#Instantiation
<https://www.ica.org/standards/RiC/ontology#Instantiation> rdf:type owl:Class ;
                                                           rdfs:subClassOf <https://www.ica.org/standards/RiC/ontology#Thing> ;
                                                           rdfs:comment """The inscription of information made by an Agent on a physical
            carrier in any persistent, recoverable form as a means of communicating information
            through time and space."""@en ;
                                                           rdfs:isDefinedBy <https://www.ica.org/standards/RiC/ontology> ;
                                                           rdfs:label "Instanciación"@es ,
                                                                      "Instanciation"@fr ,
                                                                      "Instantiation"@en ;
                                                           <http://www.w3.org/2004/02/skos/core#changeNote> [ ] ,
[ ] ,
[ ] ,
[ ] ;
<http://www.w3.org/2004/02/skos/core#scopeNote> """A Record or Record Part must have been instantiated at least
            once, though this instantiation may no longer exist at the moment of description. An
            instantiation might also exist at the moment of description, but be destroyed at a later
            moment in time, when, for example, a derived instantiation might become the only
            remaining instantiation. A Record Set may have an instantiation, which is to say that it
            is not a necessary condition. An Instantiation may be derived from another
            Instantiation. A Record Resource may have many Instantiations simultaneously (for
            instance, a record printed and saved in the same time as DOCX and PDF/A would have 3
            concurrent instantiations) or through time (for example, copy of a record). Depending on
            the context, a new instantiation may be seen as a new or as the same record resource.
            During in the process of re-instantiation something is lost and something is preserved,
            but it is up to the context and the Agent that produces or uses that Instantiation to
            assess whether the two instantiations are functionally equivalent or not. For instance,
            a postcard representing a town map from 1874 (Instantiation 1) is digitized and kept as
            a JPEG file (Instantiation 2). The digital copy may be considered as instantiating the
            \"same\" Record by an Agent considering the information transmitted by the Record (e.g.,
            the urban landscape displayed), but as a\" different\" Record by an antiquarian more
            focused on the materiality of the carrier. Successive instantiations may change the
            perceivable boundaries of a Record Resource. For instance, a case file comprising many
            records may be digitized and saved as one single PDF file, which, from management
            perspective, may be treated as one Record. Similarly, a large Record Set (a fonds or a
            series) may be maintained as one database. On the other hand, one record (main document
            and its annexes) may be digitized in separate files and each one may be managed as a
            discrete “physical” item. Instantiations may require mediation to communicate the
            information in the Record Resource. While a traditional Record on paper can simply be
            read by an Agent in order to understand the information, a vinyl recording, a video
            cassette or a digital file needs a device (mediator) to codify or decodify the
            information conveyed. This mediator may imply simple physical components (a turntable
            needle, for example), or a complex gallery of software and hardware elements.
            Instantiations are more than the mere informational content of Record Resource and may
            be the focus of preservation and physical management of records. The use of particular
            document types for records, such as a medieval charter, may have implications for the
            authenticity of the records. Hence, the way a Record Resource is instantiated
            contributes to the contextualizing of the content.record resource is instantiated
            contributes to the contextualizing the content. Distinguishing the message conveyed
            (Record Resource) and its physical representations (Instantiation) allows for the
            efficient management of their descriptions, and preserve information about a Record
            Resource even when no physical representation of it exists or is known to exist anymore.
            The relations between distinct instantiations can then be expressed wherever they
            coexist, and they can be related to the Record Resource they
            instantiate."""@en ;
<https://www.ica.org/standards/RiC/ontology#RiCCMCorrespondingComponent> """Corresponds to RiC-E06 (Instantiation
            entity)"""@en ;
<https://www.ica.org/standards/RiC/ontology#closeTo> "PREMIS Representation"@en .


###  https://www.ica.org/standards/RiC/ontology#Language
<https://www.ica.org/standards/RiC/ontology#Language> rdf:type owl:Class ;
                                                      rdfs:subClassOf <https://www.ica.org/standards/RiC/ontology#Concept> ;
                                                      rdfs:comment """A spoken or written human language represented in a Record
            Resource or used by an Agent."""@en ;
                                                      rdfs:isDefinedBy <https://www.ica.org/standards/RiC/ontology> ;
                                                      rdfs:label "Language"@en ,
                                                                 "Langue"@fr ,
                                                                 "Lengua"@es ;
                                                      <http://www.w3.org/2004/02/skos/core#changeNote> [ ] ,
[ ] ,
[ ] ,
[ ] ,
[ ] ;
<https://www.ica.org/standards/RiC/ontology#RiCCMCorrespondingComponent> """Corresponds to RiC-A25 (Language
            attribute)"""@en .


###  https://www.ica.org/standards/RiC/ontology#Mechanism
<https://www.ica.org/standards/RiC/ontology#Mechanism> rdf:type owl:Class ;
                                                       owl:disjointWith <https://www.ica.org/standards/RiC/ontology#Person> .


###  https://www.ica.org/standards/RiC/ontology#Name
<https://www.ica.org/standards/RiC/ontology#Name> rdf:type owl:Class ;
                                                  rdfs:subClassOf <https://www.ica.org/standards/RiC/ontology#Appellation> ;
                                                  rdfs:comment """A label, title or term designating an entity in order to make it
            distinguishable from other similar entities."""@en ;
                                                  rdfs:isDefinedBy <https://www.ica.org/standards/RiC/ontology> ;
                                                  rdfs:label "Name"@en ,
                                                             "Nom"@fr ,
                                                             "Nombre"@es ;
                                                  <http://www.w3.org/2004/02/skos/core#changeNote> [ ] ,
[ ] ,
[ ] ;
<http://www.w3.org/2004/02/skos/core#scopeNote> """Provides brief information about the content or other
            individual characteristics of the entity being described, necessary to distinguish it
            from other perhaps similar entities."""@en ;
<https://www.ica.org/standards/RiC/ontology#RiCCMCorrespondingComponent> """Class implementation of RiC-A28 (Name attribute)
            (see also the name datatype property)"""@en .


###  https://www.ica.org/standards/RiC/ontology#PerformanceRelation
<https://www.ica.org/standards/RiC/ontology#PerformanceRelation> rdf:type owl:Class ;
                                                                 owl:equivalentClass [ rdf:type owl:Restriction ;
                                                                                       owl:onProperty <https://www.ica.org/standards/RiC/ontology#performanceRelation_role> ;
                                                                                       owl:hasSelf "true"^^xsd:boolean
                                                                                     ] ;
                                                                 rdfs:subClassOf <https://www.ica.org/standards/RiC/ontology#EventRelation> ,
                                                                                 [ rdf:type owl:Restriction ;
                                                                                   owl:onProperty <https://www.ica.org/standards/RiC/ontology#relationHasSource> ;
                                                                                   owl:minQualifiedCardinality "1"^^xsd:nonNegativeInteger ;
                                                                                   owl:onClass <https://www.ica.org/standards/RiC/ontology#Activity>
                                                                                 ] ,
                                                                                 [ rdf:type owl:Restriction ;
                                                                                   owl:onProperty <https://www.ica.org/standards/RiC/ontology#relationHasTarget> ;
                                                                                   owl:minQualifiedCardinality "1"^^xsd:nonNegativeInteger ;
                                                                                   owl:onClass <https://www.ica.org/standards/RiC/ontology#Agent>
                                                                                 ] ;
                                                                 rdfs:comment """Connects at least one Activity to at least one Agent that
            performs or performed the activity. The Activity(-ies) is the source of the Relation and
            the Agent(s) is the target."""@en ;
                                                                 rdfs:isDefinedBy <https://www.ica.org/standards/RiC/ontology> ;
                                                                 rdfs:label "Performance Relation"@en ,
                                                                            "Relación de desarrollo funcional"@es ,
                                                                            "Relation entre activités et agents"@fr ;
                                                                 <http://www.w3.org/2004/02/skos/core#changeNote> [ ] ,
[ ] ,
[ ] ,
[ ] ,
[ ] ;
<https://www.ica.org/standards/RiC/ontology#RiCCMCorrespondingComponent> """Class implementation of RiC-R060 and RiC-R060i
            relations"""@en .


###  https://www.ica.org/standards/RiC/ontology#Person
<https://www.ica.org/standards/RiC/ontology#Person> rdf:type owl:Class ;
                                                    rdfs:subClassOf <https://www.ica.org/standards/RiC/ontology#Agent> ;
                                                    owl:disjointWith <https://www.ica.org/standards/RiC/ontology#Position> ;
                                                    rdfs:comment "An individual human being."@en ;
                                                    rdfs:isDefinedBy <https://www.ica.org/standards/RiC/ontology> ;
                                                    rdfs:label "Person"@en ,
                                                               "Persona"@es ,
                                                               "Personne"@fr ;
                                                    <http://www.w3.org/2004/02/skos/core#changeNote> [ ] ,
[ ] ,
[ ] ,
[ ] ,
[ ] ,
[ ] ,
[ ] ;
<http://www.w3.org/2004/02/skos/core#scopeNote> """Person is a kind of Agent. Most commonly, a human being
            (biological person) has a single socially constructed identity or persona. Less common
            though not rare, one or more personae in addition to the original persona which emerges
            at or near birth may be associated with the human being over the course of that human
            being’s lifetime. Such \"alternative personae\" are most often created by the original
            person for specific purposes. The original persona may, in everyday discourse, be
            regarded as “the real person”. Under some circumstances, an alternative persona might
            eclipse or replace the original person (Mark Twain eclipsing Samuel Clemens; John Wayne
            eclipsing Marion Mitchell Morrison), that is, the alternative identity becomes the
            predominant identity. Less common is when two or more persons collaborate to create a
            shared persona. A persona shared by two or more persons constitutes a kind of group.
            Within the archival context, the description of a person commonly will focus on the
            original associated persona, with alternative personae noted. Exceptionally, an
            alternative persona may displace the original persona as the focus of the description.
            Under some circumstances, for example, when record resources are associated with two or
            more different personae of one person, describing the different personae as separate
            though related persons may be desirable. Alternatively, a person may change their
            identity over the course of their lifetime."""@en ;
<https://www.ica.org/standards/RiC/ontology#RiCCMCorrespondingComponent> """Corresponds to RiC-E08 (Person
            entity)"""@en .


###  https://www.ica.org/standards/RiC/ontology#PhysicalLocation
<https://www.ica.org/standards/RiC/ontology#PhysicalLocation> rdf:type owl:Class ;
                                                              rdfs:subClassOf <https://www.ica.org/standards/RiC/ontology#Thing> ;
                                                              rdfs:comment """A delimitation of the physical territory of a
            Place."""@en ;
                                                              rdfs:isDefinedBy <https://www.ica.org/standards/RiC/ontology> ;
                                                              rdfs:label "Localisation physique"@fr ,
                                                                         "Localización física de lugar"@es ,
                                                                         "Physical Location"@en ;
                                                              <http://www.w3.org/2004/02/skos/core#changeNote> [ ] ,
[ ] ,
[ ] ,
[ ] ;
<http://www.w3.org/2004/02/skos/core#scopeNote> """Used to describe basic human-readable text such as an address,
            a cadastral reference, or less precise information found in a record. Use the
            coordinates datatype property, or the Coordinates class to capture the geographical
            coordinates of the Place. Use spatial relations (particularly 'has or had location') to
            capture a relation between two places."""@en ;
<https://www.ica.org/standards/RiC/ontology#RiCCMCorrespondingComponent> """Class implementation of RiC-A27 (Location
            attribute)"""@en .


###  https://www.ica.org/standards/RiC/ontology#Place
<https://www.ica.org/standards/RiC/ontology#Place> rdf:type owl:Class ;
                                                   rdfs:subClassOf <https://www.ica.org/standards/RiC/ontology#Thing> ;
                                                   rdfs:comment "Bounded, named geographic area or region."@en ;
                                                   rdfs:isDefinedBy <https://www.ica.org/standards/RiC/ontology> ;
                                                   rdfs:label "Lieu"@fr ,
                                                              "Lugar"@es ,
                                                              "Place"@en ;
                                                   <http://www.w3.org/2004/02/skos/core#changeNote> [ ] ,
[ ] ,
[ ] ,
[ ] ,
[ ] ;
<http://www.w3.org/2004/02/skos/core#scopeNote> """A jurisdiction is the bounded geographic area within which an
            Agent has the authority to perform specified activities constrained by rules.
            Jurisdictions, man-made structures, and natural features are historical entities. A
            Place thus may have a beginning date and ending date and changing boundaries that result
            from human or natural events. A Place may be systematically referenced to a location on
            the earth (geographic coordinates)."""@en ;
<https://www.ica.org/standards/RiC/ontology#RiCCMCorrespondingComponent> """Corresponds to RiC-E22 (Place
            entity)"""@en .


###  https://www.ica.org/standards/RiC/ontology#PlaceType
<https://www.ica.org/standards/RiC/ontology#PlaceType> rdf:type owl:Class ;
                                                       rdfs:subClassOf <https://www.ica.org/standards/RiC/ontology#Type> ;
                                                       rdfs:comment "Categorization of a Place."@en ;
                                                       rdfs:isDefinedBy <https://www.ica.org/standards/RiC/ontology> ;
                                                       rdfs:label "Place Type"@en ,
                                                                  "Tipo de lugar"@es ,
                                                                  "Type de lieu"@fr ;
                                                       <http://www.w3.org/2004/02/skos/core#changeNote> [ ] ,
[ ] ,
[ ] ;
<http://www.w3.org/2004/02/skos/core#scopeNote> """Broadly, a Place may be a member of three broad categories:
            jurisdiction, manmade structure, or a natural feature. Each of these three categories
            can subdivided into narrower categories."""@en ;
<https://www.ica.org/standards/RiC/ontology#RiCCMCorrespondingComponent> """Corresponds to RiC-A32 (Place Type
            attribute)"""@en .


###  https://www.ica.org/standards/RiC/ontology#Position
<https://www.ica.org/standards/RiC/ontology#Position> rdf:type owl:Class .


###  https://www.ica.org/standards/RiC/ontology#Record
<https://www.ica.org/standards/RiC/ontology#Record> rdf:type owl:Class .


###  https://www.ica.org/standards/RiC/ontology#RecordPart
<https://www.ica.org/standards/RiC/ontology#RecordPart> rdf:type owl:Class .


###  https://www.ica.org/standards/RiC/ontology#RecordResource
<https://www.ica.org/standards/RiC/ontology#RecordResource> rdf:type owl:Class .


###  https://www.ica.org/standards/RiC/ontology#RecordResourceToInstantiationRelation
<https://www.ica.org/standards/RiC/ontology#RecordResourceToInstantiationRelation> rdf:type owl:Class ;
                                                                                   owl:equivalentClass [ rdf:type owl:Restriction ;
                                                                                                         owl:onProperty <https://www.ica.org/standards/RiC/ontology#recordResourceToInstantiationRelation_role> ;
                                                                                                         owl:hasSelf "true"^^xsd:boolean
                                                                                                       ] ;
                                                                                   rdfs:subClassOf <https://www.ica.org/standards/RiC/ontology#Relation> ,
                                                                                                   [ rdf:type owl:Restriction ;
                                                                                                     owl:onProperty <https://www.ica.org/standards/RiC/ontology#relationHasTarget> ;
                                                                                                     owl:minQualifiedCardinality "1"^^xsd:nonNegativeInteger ;
                                                                                                     owl:onClass <https://www.ica.org/standards/RiC/ontology#Instantiation>
                                                                                                   ] ,
                                                                                                   [ rdf:type owl:Restriction ;
                                                                                                     owl:onProperty <https://www.ica.org/standards/RiC/ontology#relationHasSource> ;
                                                                                                     owl:qualifiedCardinality "1"^^xsd:nonNegativeInteger ;
                                                                                                     owl:onClass <https://www.ica.org/standards/RiC/ontology#RecordResource>
                                                                                                   ] ;
                                                                                   rdfs:comment """Connects a Record Resource to one or more Instantiations that
            instantiate it, and which either may exist or may have been lost or destroyed. The
            Record Resource is the source of the Relation and the Instantiation(s) is the
            target."""@en ;
                                                                                   rdfs:isDefinedBy <https://www.ica.org/standards/RiC/ontology> ;
                                                                                   rdfs:label "Record Resource to Instantiation Relation"@en ,
                                                                                              "Relación de recurso documental a instanciación"@es ,
                                                                                              "Relation d’instanciation"@fr ;
                                                                                   <http://www.w3.org/2004/02/skos/core#changeNote> [ ] ,
[ ] ,
[ ] ,
[ ] ,
[ ] ;
<http://www.w3.org/2004/02/skos/core#scopeNote> """In some situations, it may be useful or necessary to connect a
            record resource to an instantiation that no longer exists or has been lost, when some of
            its characteristics are known from a source, such as an old finding
            aid."""@en ;
<https://www.ica.org/standards/RiC/ontology#RiCCMCorrespondingComponent> """Class implementation of RiC-R025 and RiC-R025i
            relations"""@en .


###  https://www.ica.org/standards/RiC/ontology#Relation
<https://www.ica.org/standards/RiC/ontology#Relation> rdf:type owl:Class .


###  https://www.ica.org/standards/RiC/ontology#RoleType
<https://www.ica.org/standards/RiC/ontology#RoleType> rdf:type owl:Class ;
                                                      rdfs:subClassOf <https://www.ica.org/standards/RiC/ontology#Type> ;
                                                      rdfs:comment """The role an Agent plays in some context (usually in some
            creation relation). Not to be confused with a Position (position of an agent in some
            group). For example, a Person who is the head of some Corporate Body may play the role
            of annotator (of a record) in a creation relation."""@en ;
                                                      rdfs:isDefinedBy <https://www.ica.org/standards/RiC/ontology> ;
                                                      rdfs:label "Role Type"@en ,
                                                                 "Tipo de rol"@es ,
                                                                 "Type de rôle"@fr ;
                                                      <http://www.w3.org/2004/02/skos/core#changeNote> [ ] ,
[ ] .


###  https://www.ica.org/standards/RiC/ontology#SequentialRelation
<https://www.ica.org/standards/RiC/ontology#SequentialRelation> rdf:type owl:Class .


###  https://www.ica.org/standards/RiC/ontology#TemporalRelation
<https://www.ica.org/standards/RiC/ontology#TemporalRelation> rdf:type owl:Class ;
                                                              owl:equivalentClass [ rdf:type owl:Restriction ;
                                                                                    owl:onProperty <https://www.ica.org/standards/RiC/ontology#temporalRelation_role> ;
                                                                                    owl:hasSelf "true"^^xsd:boolean
                                                                                  ] ;
                                                              rdfs:subClassOf <https://www.ica.org/standards/RiC/ontology#SequentialRelation> ,
                                                                              [ rdf:type owl:Restriction ;
                                                                                owl:onProperty <https://www.ica.org/standards/RiC/ontology#relationHasSource> ;
                                                                                owl:minQualifiedCardinality "1"^^xsd:nonNegativeInteger ;
                                                                                owl:onClass <https://www.ica.org/standards/RiC/ontology#Thing>
                                                                              ] ,
                                                                              [ rdf:type owl:Restriction ;
                                                                                owl:onProperty <https://www.ica.org/standards/RiC/ontology#relationHasTarget> ;
                                                                                owl:minQualifiedCardinality "1"^^xsd:nonNegativeInteger ;
                                                                                owl:onClass <https://www.ica.org/standards/RiC/ontology#Thing>
                                                                              ] ;
                                                              rdfs:comment """Connects at least one Thing to at least one other Thing that
            follows it in chronological order. The Relation is oriented chronologically: the
            preceding Thing(s) is the source of the Relation, the following Thing(s) is the
            target."""@en ;
                                                              rdfs:isDefinedBy <https://www.ica.org/standards/RiC/ontology> ;
                                                              rdfs:label "Relación temporal"@es ,
                                                                         "Relation temporelle"@fr ,
                                                                         "Temporal Relation"@en ;
                                                              <http://www.w3.org/2004/02/skos/core#changeNote> [ ] ,
[ ] ,
[ ] ,
[ ] ,
[ ] ;
<http://www.w3.org/2004/02/skos/core#scopeNote> """There may be zero to many intermediate entities, ignored or
            unknown, in the chronological sequence between the connected entities."""@en ;
<https://www.ica.org/standards/RiC/ontology#RiCCMCorrespondingComponent> """Class implementation of RiC-R009 and RiC-R009i
            relations"""@en .


###  https://www.ica.org/standards/RiC/ontology#Thing
<https://www.ica.org/standards/RiC/ontology#Thing> rdf:type owl:Class .


###  https://www.ica.org/standards/RiC/ontology#Type
<https://www.ica.org/standards/RiC/ontology#Type> rdf:type owl:Class .


###  Generated by the OWL API (version 4.5.9.2019-02-01T07:24:44Z) https://github.com/owlcs/owlapi
